More work on the Tauto tactic.

examples/Tauto/Tauto.v
@@ -1,11 +1,16 @@
 Require Import Coq.Lists.List.
-Require Import MirrorCore.MTypes.ModularTypes.
-Require Import MirrorCore.Lambda.ExprCore.
+Require Import Coq.Bool.Bool.
+
+Require Import ExtLib.Core.RelDec.
+
 Require Import McExamples.Tauto.MSimpleTyp.
 Require Import McExamples.Tauto.ILogic.
 Require Import McExamples.Tauto.ILogicFunc.
 Require Import McExamples.Tauto.ILogicReify.
 
+Require Import MirrorCore.Lambda.Red.
+Require Import MirrorCore.MTypes.ModularTypes.
+Require Import MirrorCore.Lambda.ExprCore.
 Require Import MirrorCore.PLemma.
 Require Import MirrorCore.RTac.PApply.
 Require Import MirrorCore.Lemma.
@@ -16,8 +21,38 @@ Require Import MirrorCore.RTac.RTac.
 Definition tc (t : typ) :=
   match t with
     | ModularTypes.tyProp => true
-    | _ => true
+    | _ => false
   end.
+
+Require Import MirrorCore.Reify.Reify.
+Require Import MirrorCore.Reify.ReifyClass.
+
+Definition test : (lemma typ (expr typ ilfunc) (expr typ ilfunc)) :=
+  Eval unfold Lemma.add_var, Lemma.add_prem , Lemma.vars , Lemma.concl , Lemma.premises in
+  <:: @limplAdj Prop _ _ ::>.
+
+Print test.
+Check limplAdj.
+
+Definition conclD (us vs : tenv typ) (e : expr typ ilfunc) : option (exprT us vs Prop) :=
+  exprD us vs tyProp e.
+
+Definition r_refl : PolyLemma typ (expr typ ilfunc) (expr typ ilfunc) :=
+  {| p_n := 1;
+     p_lem := fun t => 
+               {| vars := t :: nil;
+                  premises := nil;
+                  concl := App (App (Inj (fEntails t)) (Var 0)) (Var 0) |};
+     p_tc := tc
+  |}.
+
+Lemma r_refl_sound : PolyLemmaD conclD r_refl.
+Proof.
+  unfold PolyLemmaD, with_typeclasses; simpl.
+  destruct t; simpl in *; try apply I.
+  unfold lemmaD; simpl; intros.
+  intro H; apply H.
+Qed.
 
 Definition r_trueR : PolyLemma typ (expr typ ilfunc) (expr typ ilfunc) :=
   {| p_n := 1;
@@ -27,6 +62,16 @@ Definition r_trueR : PolyLemma typ (expr typ ilfunc) (expr typ ilfunc) :=
                   concl := App (App (Inj (fEntails t)) (Var 0)) (mkTrue t) |};
      p_tc := tc
   |}.
+
+Lemma r_trueR_sound : PolyLemmaD conclD r_trueR.
+Proof.
+  unfold PolyLemmaD, with_typeclasses; simpl.
+  destruct t; simpl in *; try apply I.
+  unfold lemmaD; simpl; intros.
+  unfold AbsAppI.exprT_App, exprT_Inj; simpl.
+  unfold entailsR, castR; simpl; intros.
+  apply I.
+Qed.
 
 Definition r_falseL : PolyLemma typ (expr typ ilfunc) (expr typ ilfunc) :=
   {| p_n := 1;
@@ -40,7 +85,7 @@ Definition r_falseL : PolyLemma typ (expr typ ilfunc) (expr typ ilfunc) :=
 Definition r_andR : PolyLemma typ (expr typ ilfunc) (expr typ ilfunc) :=
   {| p_n := 1;
      p_lem := fun t => 
-               {| vars := t :: nil;
+               {| vars := t :: t :: t :: nil;
                   premises := App (App (Inj (fEntails t)) (Var 0)) (Var 2)
                                   :: App (App (Inj (fEntails t)) (Var 0)) (Var 1) :: nil;
                   concl := App (App (Inj (fEntails t)) (Var 0))
@@ -48,20 +93,131 @@ Definition r_andR : PolyLemma typ (expr typ ilfunc) (expr typ ilfunc) :=
      p_tc := tc
   |}.
 
+Definition r_andL1 : PolyLemma typ (expr typ ilfunc) (expr typ ilfunc) :=
+  {| p_n := 1;
+     p_lem := fun t => 
+               {| vars := t :: t :: t :: nil;
+                  premises := App (App (Inj (fEntails t)) (Var 2))
+                                  (Var 0) :: nil;
+                  concl := App
+                             (App (Inj (fEntails t))
+                                  (App (App (Inj (fAnd t)) (Var 2))
+                                       (Var 1))) (Var 0) |};
+     p_tc := tc
+  |}.
+
+Definition r_andL2 : PolyLemma typ (expr typ ilfunc) (expr typ ilfunc) :=
+  {| p_n := 1;
+     p_lem := fun t => 
+               {| vars := t :: t :: t :: nil;
+                  premises := App (App (Inj (fEntails t)) (Var 1))
+                                  (Var 0) :: nil;
+                  concl := App
+                             (App (Inj (fEntails t))
+                                  (App (App (Inj (fAnd t)) (Var 2))
+                                       (Var 1))) (Var 0) |};
+     p_tc := tc
+  |}.
+
+Definition r_orL : PolyLemma typ (expr typ ilfunc) (expr typ ilfunc) :=
+  {| p_n := 1;
+     p_lem := fun t => 
+               {| vars := t :: t :: t :: nil;
+                  premises := App (App (Inj (fEntails t)) (Var 2))
+                                  (Var 0)
+                              :: App (App (Inj (fEntails t)) (Var 1))
+                              (Var 0) :: nil;
+                  concl := App
+                             (App (Inj (fEntails t))
+                                  (App (App (Inj (fOr t)) (Var 2)) (Var 1)))
+                             (Var 0) |};
+     p_tc := tc
+  |}.
+
+Definition r_orR1 : PolyLemma typ (expr typ ilfunc) (expr typ ilfunc) :=
+  {| p_n := 1;
+     p_lem := fun t => 
+               {| vars := t :: t :: t :: nil;
+                  premises := App (App (Inj (fEntails t)) (Var 0))
+                                  (Var 2) :: nil;
+                  concl := App (App (Inj (fEntails t)) (Var 0))
+                               (App (App (Inj (fOr t)) (Var 2)) (Var 1)) |};
+     p_tc := tc
+  |}.
+
+Definition r_orR2 : PolyLemma typ (expr typ ilfunc) (expr typ ilfunc) :=
+  {| p_n := 1;
+     p_lem := fun t => 
+               {| vars := t :: t :: t :: nil;
+                  premises := App (App (Inj (fEntails t)) (Var 0))
+                                  (Var 1) :: nil;
+                  concl := App (App (Inj (fEntails t)) (Var 0))
+                               (App (App (Inj (fOr t)) (Var 2)) (Var 1)) |};
+     p_tc := tc
+  |}.
+
+Definition r_implAdj : PolyLemma typ (expr typ ilfunc) (expr typ ilfunc) :=
+  {| p_n := 1;
+     p_lem := fun t => 
+               {| vars := t :: t :: t :: nil;
+                  premises := App
+                                (App (Inj (fEntails t))
+                                     (App (App (Inj (fAnd t)) (Var 0))
+                                          (Var 2))) (Var 1) :: nil;
+                  concl := App (App (Inj (fEntails t)) (Var 0))
+                               (App (App (Inj (fImpl t)) (Var 2)) (Var 1)) |};
+     p_tc := tc
+  |}.
+
+
 Definition PAPPLY (plem : PolyLemma typ (expr typ ilfunc) (expr typ ilfunc)) :=
   PAPPLY 
     (fun subst SS SU tus tvs n l r t s =>
               @exprUnify subst typ ilfunc RType_typ RSym_ilfunc Typ2_Fun
                          SS SU 10 tus tvs n l r t s) plem.
 
+Definition fintro (e : expr typ ilfunc) : option (@OpenAs typ (expr typ ilfunc)) :=
+  match e with
+  | App (App (Inj (ilf_entails t1)) P) (App (Inj (ilf_exists t2 t3)) Q) =>
+    if t1 ?[eq] t3 && tc t1 then
+      Some (AsEx t2 (fun x => beta (App Q x)))
+    else
+      None
+  | App (App (Inj (ilf_entails t1)) (App (Inj (ilf_forall t2 t3)) P)) Q =>
+    if t1 ?[eq] t3 && tc t1 then
+      Some (AsEx t2 (fun x => beta (App P x)))
+    else
+      None
+  | App (App (Inj (ilf_entails t1)) (App (Inj (ilf_exists t2 t3)) P)) Q =>
+    if t1 ?[eq] t3 && tc t1 then
+      Some (AsAl t2 (fun x => beta (App P x)))
+    else
+      None
+  | App (App (Inj (ilf_entails t1)) P) (App (Inj (ilf_forall t2 t3)) Q) =>
+    if t1 ?[eq] t3 && tc t1 then
+      Some (AsAl t2 (fun x => beta (App Q x)))
+    else
+      None
+  | _ => None
+  end.
+
+Definition INTRO := @INTRO typ (expr typ ilfunc) ExprVar_expr ExprUVar_expr fintro.
 
 Definition TAUTO : rtac typ (expr typ ilfunc) :=
   REC 10
       (fun r =>
-         (FIRST
-            (PAPPLY r_trueR ::
-             PAPPLY r_falseL :: 
-             THEN (PAPPLY r_andR) (runOnGoals r) :: nil))) FAIL.
+         THEN (REPEAT 10 INTRO) 
+              (runOnGoals 
+                 (FIRST
+                    (PAPPLY r_trueR ::
+                     PAPPLY r_falseL :: 
+                     PAPPLY r_refl :: 
+                     THEN (PAPPLY r_andR) (runOnGoals r) :: 
+                     THEN (PAPPLY r_orL) (runOnGoals r) :: 
+                     SOLVE (THEN (PAPPLY r_orR1) (runOnGoals r)) :: 
+                     SOLVE (THEN (PAPPLY r_orR2) (runOnGoals r)) :: 
+                     SOLVE (THEN (PAPPLY r_andL1) (runOnGoals r)) :: 
+                     SOLVE (THEN (PAPPLY r_andL2) (runOnGoals r)) :: nil)))) FAIL.
 
 Goal True.
 pose (PApply.get_lemma r_trueR
