theories/PLemma.v
@@ -1,3 +1,4 @@
+Require Import MirrorCore.ExprI.
 Require Import MirrorCore.Lemma.
 Require Import MirrorCore.Polymorphic.
 
@@ -13,3 +14,28 @@ Section PolyLemma.
 End PolyLemma.
 
 Arguments PolyLemma : clear implicits.
+
+Section PolyLemmaD.
+  Context {typ expr conclusion : Type}.
+  Context {RType_typ : RType typ}.
+  Context {Expr_expr : Expr _ expr}.
+
+  Context {Typ0_Prop : Typ0 RType_typ Prop}.
+ 
+  Variable conclusionD : forall us vs, conclusion -> option (exprT us vs Prop).
+
+  Definition with_typeclasses {T : Type} (TD : T -> Prop) {n}
+             (tc : polymorphic typ n bool) (pc : polymorphic typ n T)
+    : polymorphic typ n Prop :=
+    make_polymorphic (fun args =>
+                        if inst tc args
+                        then TD (inst pc args)
+                        else True).
+
+  Definition PolyLemmaD plem :=
+    polymorphicD (fun x => x) 
+                 (with_typeclasses (lemmaD conclusionD nil nil) 
+                                   (p_tc plem) 
+                                   (p_lem plem)).
+
+End PolyLemmaD.
